Cook_Levin/IMP-_To_SAS+/IMP-_To_IMP--/Binary_Arithmetic_IMP.thy
@@ -1,0 +1,205 @@
+theory Binary_Arithmetic_IMP 
+  imports "../../../IMP-/IMP_Minus_Nat_Bijection"  Binary_Arithmetic_Nat
+begin
+
+unbundle IMP_Minus_Minus_Com.no_com_syntax
+unbundle Com.no_com_syntax
+
+fun nth_bit_of_num_nat :: "nat \<Rightarrow> nat \<Rightarrow> nat" where
+"nth_bit_of_num_nat x n  = (if x = 0 then (if n = 0 then 1 else 0) else
+                            if n = 0 then (if hd_nat x = 0 then 0 else 1) else
+                            nth_bit_of_num_nat (tl_nat x) (n-1)) "
+
+definition nth_bit_of_num_if ::pcom where "nth_bit_of_num_if \<equiv>
+ IF ''x''\<noteq>0 THEN 
+        (IF ''n''\<noteq>0 THEN ''b''::= A (N 1) ELSE ''b''::= A (N 0)) 
+        ELSE ''b''::= A (N 0) 
+"
+
+abbreviation nth_bit_of_num_if_state_transformer 
+  where "nth_bit_of_num_if_state_transformer p x n \<equiv>
+    state_transformer p [(''b'',if x >0 \<and> n>0 then 1 else 0)]
+"
+
+fun nth_bit_of_num_if_time :: "nat \<Rightarrow> nat \<Rightarrow> nat" where 
+"nth_bit_of_num_if_time 0 _ = 3"|
+"nth_bit_of_num_if_time _ _ = 4"
+
+lemma nth_bit_of_num_if_correct[intro]:
+"\<lbrakk> s (add_prefix p ''x'')= x ; s (add_prefix p ''n'') = n  \<rbrakk> \<Longrightarrow>
+(nth_bit_of_num_if p, s) \<Rightarrow>\<^bsup>nth_bit_of_num_if_time x n \<^esup>
+nth_bit_of_num_if_state_transformer p x n s "
+  unfolding nth_bit_of_num_if_def 
+  apply (cases x;cases n)
+     apply (rule Big_StepT.IfFalse)
+       apply simp
+      apply (rule terminates_in_time_state_intro)
+        apply blast
+       apply simp
+      apply simp
+     apply simp
+ apply (rule Big_StepT.IfFalse)
+       apply simp
+      apply (rule terminates_in_time_state_intro)
+        apply blast
+       apply simp
+      apply simp
+    apply simp
+   apply (rule Big_StepT.IfTrue)
+     apply simp
+    apply (rule Big_StepT.IfFalse)
+      apply simp
+        apply (rule terminates_in_time_state_intro)
+       apply fast
+      apply fast
+     apply force
+    apply simp
+   apply simp
+      apply (rule Big_StepT.IfTrue)
+    apply simp
+            apply (rule Big_StepT.IfTrue)
+     apply simp
+              apply (rule terminates_in_time_state_intro)
+  apply blast
+     apply simp
+    apply simp
+  apply simp
+  by simp
+  
+definition nth_bit_of_num_iteration::pcom  where "nth_bit_of_num_iteration \<equiv>
+
+  [''tl''] ''xs'' ::=  (A ( V ''x'')) ;;
+   invoke_subprogram ''tl'' tl_IMP;;
+   ''x'' ::= [''tl''] (A (V ''ans''));;
+   ''n'' ::= (V ''n'' \<ominus> N 1 );; 
+    nth_bit_of_num_if
+"
+
+definition nth_bit_of_num_iteration_t :: "nat \<Rightarrow> nat \<Rightarrow> nat" where 
+"nth_bit_of_num_iteration_t x n = 6 + tl_time x + nth_bit_of_num_if_time (tl_nat x) (n-1)"
+
+abbreviation nth_bit_of_num_iteration_state_transformer 
+  where "nth_bit_of_num_iteration_state_transformer p x n \<equiv>
+    state_transformer p [(''x'', tl_nat x),(''n'',n-1)] o tl_state_transformer (''tl'' @ p) x
+  o nth_bit_of_num_if_state_transformer p (tl_nat x) (n-1)
+"
+value "nth_bit_of_num_iteration_state_transformer"
+lemma nth_bit_of_num_iteration_correct[intro]:
+ " s (add_prefix p ''x'') = x \<Longrightarrow> s (add_prefix p ''n'') = n \<Longrightarrow>
+(nth_bit_of_num_iteration p,s)  \<Rightarrow>\<^bsup>nth_bit_of_num_iteration_t x n \<^esup> 
+nth_bit_of_num_iteration_state_transformer p x n s"
+  unfolding nth_bit_of_num_iteration_def nth_bit_of_num_iteration_t_def
+  apply (rule terminates_in_time_state_intro)
+    apply (rule Big_StepT.Seq)+
+  by fastforce+
+
+
+definition nth_bit_of_num_loop :: "pcom" where 
+"nth_bit_of_num_loop \<equiv> WHILE ''b''\<noteq>0 DO nth_bit_of_num_iteration"
+
+fun nth_bit_of_num_loop_t:: "nat \<Rightarrow> nat \<Rightarrow> nat \<Rightarrow> nat" where 
+"nth_bit_of_num_loop_t 0 _ _  = 2 "|
+"nth_bit_of_num_loop_t (Suc b) x n  = (let x' = tl_nat x; 
+n' = n - 1 
+in ( if x'>0 \<and> n'>0 then 1 + nth_bit_of_num_iteration_t x n + nth_bit_of_num_loop_t (Suc 0) x' n'
+else 1 + nth_bit_of_num_iteration_t x n + nth_bit_of_num_loop_t 0 x' n'
+) ) "
+
+fun nth_bit_of_num_loop_state_transformer ::
+"char list \<Rightarrow> nat \<Rightarrow> nat \<Rightarrow> nat \<Rightarrow> (char list \<Rightarrow> nat) \<Rightarrow> char list \<Rightarrow> nat" where 
+"nth_bit_of_num_loop_state_transformer p 0 x n = id "|
+"nth_bit_of_num_loop_state_transformer p (Suc b) x n = (let x' = tl_nat x; n' = n-1;
+iteration = nth_bit_of_num_iteration_state_transformer p x n  in 
+(if x'>0 \<and> n'>0 then iteration o nth_bit_of_num_loop_state_transformer p (Suc 0) x' n' else
+iteration
+o nth_bit_of_num_loop_state_transformer p 0 x' n'
+ ))"
+
+lemma " (nth_bit_of_num_iteration_state_transformer p x n
+         o nth_bit_of_num_loop_state_transformer p (Suc 0) (tl_nat x) (n-1)) s = 
+      (nth_bit_of_num_loop_state_transformer p (Suc 0) (tl_nat x) (n-1)) s"
+  apply (induction p "Suc 0" "tl_nat x" "n-1" arbitrary: x n s rule:nth_bit_of_num_loop_state_transformer.induct)
+  apply auto
+fun nth_bit_of_num_loop_state_transformer' ::
+"char list \<Rightarrow> nat \<Rightarrow> nat \<Rightarrow> nat \<Rightarrow> (char list \<Rightarrow> nat) \<Rightarrow> char list \<Rightarrow> nat" where 
+"nth_bit_of_num_loop_state_transformer' p 0 x n = id "|
+"nth_bit_of_num_loop_state_transformer' p b x n = (let x' = tl_nat x; n' = n-1;
+b' = (if x'>0 \<and> n'>0 then Suc 0 else 0); iteration = nth_bit_of_num_iteration_state_transformer p x n
+ in 
+ iteration o nth_bit_of_num_loop_state_transformer' p b' x' n')"
+
+
+thm Big_StepT.WhileTrue
+
+  
+  
+
+lemma 
+"\<lbrakk>s (add_prefix p ''x'') = x ; s (add_prefix p ''n'') = n ; s (add_prefix p ''b'') = b \<rbrakk>
+\<Longrightarrow> (nth_bit_of_num_loop p,s) \<Rightarrow>\<^bsup>nth_bit_of_num_loop_t b x n \<^esup>
+      nth_bit_of_num_loop_state_transformer p b x n s"
+  unfolding nth_bit_of_num_loop_def 
+  apply(induction b x n arbitrary:s rule: nth_bit_of_num_loop_t.induct)
+  apply(rule terminates_in_time_state_intro)
+     apply (rule Big_StepT.WhileFalse)
+     apply simp
+  apply simp
+   apply simp
+      apply(rule terminates_in_time_state_intro)
+    apply (rule Big_StepT.WhileTrue)
+       apply linarith
+      apply auto[1]
+     apply (split if_splits) apply (auto simp only:)
+  oops 
+
+lemma
+"(nth_bit_of_num_loop p,s) \<Rightarrow>\<^bsup>nth_bit_of_num_loop_t (s (add_prefix p ''b''))
+ (s (add_prefix p ''x''))
+ (s (add_prefix p ''n'')) \<^esup>
+      nth_bit_of_num_loop_state_transformer p (s (add_prefix p ''b'')) (s (add_prefix p ''x''))
+  (s (add_prefix p ''n'')) s"
+  unfolding nth_bit_of_num_loop_def 
+proof(induction "(s (add_prefix p ''b''))" "s (add_prefix p ''x'')" "s (add_prefix p ''n'')" arbitrary:s rule: nth_bit_of_num_loop_t.induct)
+case (1)
+  show ?case 
+  apply(rule terminates_in_time_state_intro)
+ apply (rule Big_StepT.WhileFalse)
+   using 1  by auto
+next
+  case (2 v)
+  obtain s' where s'_def: "s' =state_transformer p
+      [(''x'', tl_nat (s (add_prefix p ''x''))), (''n'', s (add_prefix p ''n'') - Suc 0)]
+      (state_transformer (CHR ''t'' # CHR ''l'' # p)
+        [(''ans'', tl_nat (s (add_prefix p ''x''))), (''xs'', 0)]
+        (snd_nat_IMP_Minus_state_transformer
+          (CHR ''s'' # CHR ''n'' # CHR ''d'' # CHR ''t'' # CHR ''l'' # p)
+          (s (add_prefix p ''x'') - Suc 0)
+          (state_transformer p [(''b'', Suc 0)] s)))" by simp
+    show ?case 
+      apply(rule terminates_in_time_state_intro [where s'= "if  0 < tl_nat (s (add_prefix p ''x'')) \<and> 0 < s (add_prefix p ''n'') - 1 then s1 else s2"  
+     for s1 s2] )
+        apply (rule Big_StepT.WhileTrue[where 
+ y= "if  0 < tl_nat (s (add_prefix p ''x'')) \<and> 0 < s (add_prefix p ''n'') - 1 then t1 else t2"  
+     for t1 t2])
+       using 2(3) apply linarith
+           apply rule
+            apply simp
+           apply simp
+       apply(rule terminates_split_if)
+       using 2(1)[of s'] s'_def  apply force
+       using 2(2)[of s'] s'_def apply force
+         apply fastforce
+       using 2(3)[symmetric] apply auto[1]
+       apply (smt (z3) One_nat_def less_diff_conv plus_1_eq_Suc) 
+       using 2(3)[symmetric] apply (simp only:)
+       apply (subst (2) nth_bit_of_num_loop_state_transformer.simps)
+        
+       apply (afuto simp add: Let_def simp del: nth_bit_of_num_loop_state_transformer.simps(2))
+       slefdgehammer
+         apply (auto simp only:Let_def One_nat_def  comp_apply One_nat_def less_diff_conv plus_1_eq_Suc)
+       apply (auto simp)    
+       
+qed
+
+thm If_tE
+end 
