ROOT
@@ -1,4 +1,3 @@
-session Poly_Reductions_Base = HOL + sessions NREST "HOL-Real_Asymp" Landau_Symbols
+session Poly_Reductions_Base = HOL + sessions NREST "HOL-Real_Asymp" Landau_Symbols 
 
-theories 
-Polynomial_Growth_Functions Polynomial_Reductions
+
